LogRel/LemmasLR.v
@@ -17,6 +17,13 @@ Require Import Utlc.Inst.
 Require Import Omega.
 Require Import Min.
 
+Lemma lev_lateri {i W} : lev (lateri i W) = lev W - i.
+Proof.
+  induction i; unfold lev in *; simpl in *; eauto with arith.
+  rewrite IHi. omega.
+Qed.
+
+
 Section Obs.
   Lemma obs_zero {d ts tu} : Obs d 0 ts tu.
   Proof.
@@ -108,12 +115,12 @@ Section Obs.
   Lemma obs_antired {ts ts' tu tu' W' W d i j} :
     S.evaln ts ts' i →
     U.evaln tu tu' j →
-    W' ≤ W →
+    (* W' ≤ W → *)
     lev W' + min i j ≥ lev W →
     Obs d W' ts' tu' →
     Obs d W ts tu.
   Proof.
-    intros es eu fw sge obs.
+    intros es eu (* fw *) sge obs.
     destruct d; destruct W; simpl; simpl in obs; intuition.
     - cut (tu'⇓).
       + refine (U.termination_closed_under_antireductionStar _).
@@ -278,7 +285,7 @@ Section ClosedLR.
     intros es eu fw sge tr.
     unfold termrel, termrel'.
     intros Cs Cu ecs ecu cr.
-    refine (obs_antired _ _ fw sge _); eauto using S.evaln_ctx, U.ctxevaln_ctx.
+    refine (obs_antired _ _ sge _); eauto using S.evaln_ctx, U.ctxevaln_ctx.
     apply tr; auto. 
     refine (contrel_mono fw cr).
   Qed.
@@ -477,14 +484,24 @@ End OpenLR.
 
 Section TermRelZero.
 
-  Lemma valrel_in_termrel₀ {d w τ ts tu} :
-    valrel d w τ ts tu → termrel₀ d w τ ts tu.
+  Lemma valrel_in_termreli₀ {d dfc w τ ts tu} :
+    valrel d w τ ts tu → termreli₀ d dfc w τ ts tu.
   Proof.
     intros vr.
     destruct (valrel_implies_OfType vr) as [[? ?] ?].
     unfold termrel₀. simpl. 
     left. exists ts, tu.
-    eauto with eval.
+    (* why isn't this enough? *)
+    (* eauto using clos_refl_trans_1n with eval. *)
+    split; [|split]; 
+    eauto using clos_refl_trans_1n with eval; constructor.
+  Qed.
+
+  Lemma valrel_in_termrel₀ {d w τ ts tu} :
+    valrel d w τ ts tu → termrel₀ d  w τ ts tu.
+  Proof.
+    unfold termrel₀.
+    eauto using valrel_in_termreli₀.
   Qed.
 
   Lemma termrel₀_in_termrel {d w τ ts tu} :
@@ -495,11 +512,38 @@ Section TermRelZero.
     - unfold termrel, termrel'; eauto.
   Qed.
 
-  Lemma termrel₀_antired_star {ts ts' tu tu' W d τ} :
+  Lemma termreli₀_antired {ts ts' tu tu' W d dfc τ i j} dfc' :
+    dfc' + min i j ≥ dfc  →
+    S.evaln ts ts' i →
+    U.ctxevaln tu tu' j →
+    termreli₀ d dfc W τ ts' tu' →
+    termreli₀ d dfc' W τ ts tu.
+  Proof.
+    intros ineq es eu tzi.
+    destruct tzi as [(vs & vu & es' & eu' & vr)|?].
+    - left. exists vs, vu.
+      eapply stepRel_to_evalStar in es.
+      eapply stepRel_to_evalStar in eu.
+      unfold U.ctxevalStar in *.
+      eauto using evalStepTrans with eval.
+    - right. intros Cs Cu eCs eCu.
+      specialize (H Cs Cu eCs eCu).
+
+      pose proof (ctxevaln_evaln_ctx eu Cu eCu) as eu'.
+      pose proof (evaln_ctx eCs es) as es'.
+      enough (lev (lateri dfc W) + Nat.min i j ≥ lev (lateri dfc' W)) as ineq' by 
+          eapply (obs_antired es' eu' ineq' H).
+      rewrite ?lev_lateri; unfold lev.
+      omega.
+  Qed.      
+    
+      
+
+  Lemma termreli₀_antired_star {ts ts' tu tu' W d dfc τ} :
     clos_refl_trans_1n S.Tm S.eval ts ts' →
     U.ctxevalStar tu tu' →
-    termrel₀ d W τ ts' tu' →
-    termrel₀ d W τ ts tu.
+    termreli₀ d dfc W τ ts' tu' →
+    termreli₀ d dfc W τ ts tu.
   Proof.
     intros es eu tr.
     destruct tr as [(vs & vu & ess & esu & vr)|div].
@@ -510,7 +554,19 @@ Section TermRelZero.
       destruct (evalTrans_to_stepRel (evalstar_ctx Cs eCs es)) as (? & es').
       destruct (evalTrans_to_stepRel eu) as (? & eu').
       pose proof (ctxevaln_evaln_ctx eu' Cu eCu) as eu''.
-      eapply (obs_antired (W' := W) es' eu''); eauto with arith.
+      specialize (div Cs Cu eCs eCu).
+      eapply (obs_antired (W' := (lateri dfc W)) es' eu''); try assumption.
+      rewrite ?lev_lateri.
+      omega.
+  Qed.
+
+  Lemma termrel₀_antired_star {ts ts' tu tu' W d τ} :
+    clos_refl_trans_1n S.Tm S.eval ts ts' →
+    U.ctxevalStar tu tu' →
+    termrel₀ d W τ ts' tu' →
+    termrel₀ d W τ ts tu.
+  Proof.
+    eapply termreli₀_antired_star.
   Qed.
 
   Lemma termrel₀_antired_star_left {ts ts' tu W d τ} :
@@ -550,6 +606,60 @@ Section TermRelZero.
     intros. subst.
     eauto using termrel₀_ectx.
   Qed.
+
+  Lemma termrel₀_zero {d τ ts tu} :
+    termrel₀ d 0 τ ts tu.
+  Proof.
+    right.
+    intros Cs Cu eCs eCu.
+    eapply obs_zero.
+  Qed.
+
+  Lemma termreli₀_dfc_mono {d dfc dfc' w τ ts tu}:
+    termreli₀ d dfc w τ ts tu →
+    dfc ≤ dfc' →
+    termreli₀ d dfc' w τ ts tu.
+  Proof.
+    destruct 1 as [(vs & vu & ess & esu & vr)|div]; intros ineq.
+    - left. exists vs, vu. eauto. 
+    - right. intros Cs Cu eCs eCu.
+      specialize (div Cs Cu eCs eCu).
+      refine (obs_mono _ div).
+      rewrite ?lev_lateri.
+      omega.
+  Qed.
+      
+  Lemma termreli₀_ectx {d dfc w τ₁ τ₂ ts Cs tu Cu} (eCs : S.ECtx Cs) (eCu : U.ECtx Cu) :
+    termrel₀ d (lateri dfc w) τ₁ ts tu →
+    lev w ≥ dfc →
+    (∀ vs vu, valrel d (lateri dfc w) τ₁ vs vu → termreli₀ d dfc w τ₂ (S.pctx_app vs Cs) (U.pctx_app vu Cu)) →
+    termreli₀ d dfc w τ₂ (S.pctx_app ts Cs) (U.pctx_app tu Cu).
+  Proof.
+    intros trtm ineq trcont.
+    destruct trtm as [(vs & vu & ess & esu & vr)|div].
+    - specialize (trcont vs vu vr).
+      eapply termreli₀_antired_star in trcont;
+        eauto using evalstar_ctx, extend_ctxevalStar.
+    - right.
+      intros Cs' Cu' eCs' eC'.
+      rewrite <- S.pctx_cat_app.
+      rewrite <- U.pctx_cat_app.
+      eauto using S.ectx_cat, U.ectx_cat.
+  Qed.
+
+  Lemma termreli₀_ectx' {d dfc w τ₁ τ₂ ts Cs tu ts' tu' Cu} :
+    termrel₀ d (lateri dfc w) τ₁ ts tu →
+    lev w ≥ dfc →
+    (∀ vs vu, valrel d (lateri dfc w) τ₁ vs vu → termreli₀ d dfc w τ₂ (S.pctx_app vs Cs) (U.pctx_app vu Cu)) →
+    ts' = S.pctx_app ts Cs →
+    tu' = U.pctx_app tu Cu →
+    S.ECtx Cs → U.ECtx Cu →
+    termreli₀ d dfc w τ₂ ts' tu'.
+  Proof.
+    intros. subst.
+    eauto using termreli₀_ectx.
+  Qed.
+
 End TermRelZero.
 
 Ltac crushLRMatch :=
